refactor: seperate Soundness.lean

MathematicalLogic/FirstOrder/Proof.lean
@@ -1,5 +1,5 @@
 import Mathlib.Data.Set.Finite
-import MathematicalLogic.FirstOrder.Semantics
+import MathematicalLogic.FirstOrder.Syntax
 
 namespace FirstOrder.Language
 
@@ -740,73 +740,4 @@ theorem Complete.unprovable_iff (h₁ : Complete Γ) (h₂ : Consistent Γ) : Γ
 
 def Henkin (Γ : 𝓛.FormulaSet n) := ∀ p, Γ ⊢ ∃' p → ∃ (c : 𝓛.Const), Γ ⊢ p[↦ₛ c]ₚ
 
-theorem Entails.axioms : p ∈ 𝓛.Axioms → Γ ⊨ p := by
-  intro h 𝓜 ρ _
-  induction h <;> simp [Structure.interpFormula] <;> tauto
-  case forall_elim =>
-    intro h
-    rw [Structure.interpFormula_subst, Structure.Assignment.subst_single]
-    apply h
-  case forall_self =>
-    intros h u
-    simp [Formula.shift, Structure.interpFormula_subst, Structure.Assignment.subst_shift]
-    exact h
-  case eq_subst =>
-    intros h₁ h₂
-    simp [Formula.shift, Structure.interpFormula_subst, Structure.Assignment.subst_single] at *
-    rw [←h₁]; exact h₂
-
-theorem Entails.mp : Γ ⊨.{u} p ⇒ q → Γ ⊨.{u} p → Γ ⊨.{u} q := by
-  intros h₁ h₂ 𝓜 ρ h
-  apply h₁
-  · exact h
-  · apply h₂; exact h
-
-theorem soundness : Γ ⊢ p → Γ ⊨ p := by
-  intro h
-  induction h with
-  | hyp h => intros _ _ h₁; apply h₁; exact h
-  | ax h => exact Entails.axioms h
-  | mp _ _ ih₁ ih₂ => exact Entails.mp ih₁ ih₂
-
-theorem Consistent.of_satisfiable : Satisfiable Γ → Consistent Γ := by
-  intro ⟨𝓜, ρ, h₁⟩ h₂
-  apply soundness at h₂
-  apply h₂
-  exact h₁
-
-theorem Consistent.empty : Consistent (∅ : 𝓛.FormulaSet n) := by
-  apply of_satisfiable
-  exists ⟨Unit, λ _ _ => (), λ _ _ => True⟩, λ _ => ()
-  intro _ h
-  contradiction
-
-theorem Structure.theory.complete {𝓜 : 𝓛.Structure} : Complete 𝓜.theory := by
-  intro p
-  by_cases h : 𝓜 ⊨ₛ p
-  · exact Or.inl (.hyp h)
-  · exact Or.inr (.hyp h)
-
-theorem Complete.provable_iff_satisfied {𝓣 : 𝓛.Theory} {𝓜 : 𝓣.Model} :
-  Complete 𝓣 → (𝓣 ⊢ p ↔ 𝓜 ⊨ₛ p) := by
-  intro h
-  by_cases h' : 𝓣 ⊢ p <;> simp [h']
-  · apply soundness h'; exact 𝓜.satisfy_theory
-  · cases h p with
-    | inl h => contradiction
-    | inr h => apply soundness h; exact 𝓜.satisfy_theory
-
-namespace Theory
-
-abbrev theorems (𝓣 : 𝓛.Theory) : 𝓛.Theory := { p | 𝓣 ⊢ p }
-
-abbrev Decidable (𝓣 : 𝓛.Theory) := DecidablePred 𝓣.theorems
-
-theorem eq_theory_of_complete {𝓣 : 𝓛.Theory} {𝓜 : 𝓣.Model} :
-  Complete 𝓣 → 𝓣.theorems = 𝓜.theory := by
-  intro h
-  ext p
-  simp [Structure.theory]
-  rw [h.provable_iff_satisfied]
-
-end FirstOrder.Language.Theory
+end FirstOrder.Language
