MathematicalLogic.lean
@@ -4,6 +4,11 @@ import MathematicalLogic.Vector
 import MathematicalLogic.FirstOrder.Syntax
 import MathematicalLogic.FirstOrder.Semantics
 import MathematicalLogic.FirstOrder.Proof
+import MathematicalLogic.FirstOrder.Soundness
+import MathematicalLogic.FirstOrder.Completeness.Language
+import MathematicalLogic.FirstOrder.Completeness.Henkin
+import MathematicalLogic.FirstOrder.Completeness.Lindenbaum
+import MathematicalLogic.FirstOrder.Completeness.TermModel
 import MathematicalLogic.FirstOrder.Completeness.Completeness
 import MathematicalLogic.FirstOrder.Encoding
 
