MathematicalLogic/FirstOrder/Soundness.lean
@@ -1,0 +1,77 @@
+import MathematicalLogic.FirstOrder.Semantics
+import MathematicalLogic.FirstOrder.Proof
+
+namespace FirstOrder.Language
+
+variable {𝓛 : Language}
+
+theorem Entails.axioms : p ∈ 𝓛.Axioms → Γ ⊨ p := by
+  intro h 𝓜 ρ _
+  induction h <;> simp [Structure.interpFormula] <;> tauto
+  case forall_elim =>
+    intro h
+    simp [Structure.interpFormula_subst_single]
+    apply h
+  case forall_self =>
+    intro h _
+    simp [Structure.interpFormula_shift]
+    exact h
+  case eq_subst =>
+    intro h₁ h₂
+    simp [Structure.interpFormula_subst_single] at *
+    rw [←h₁]; exact h₂
+
+theorem Entails.mp : Γ ⊨.{u} p ⇒ q → Γ ⊨.{u} p → Γ ⊨.{u} q := by
+  intros h₁ h₂ 𝓜 ρ h
+  apply h₁
+  · exact h
+  · apply h₂; exact h
+
+theorem soundness : Γ ⊢ p → Γ ⊨ p := by
+  intro h
+  induction h with
+  | hyp h => intros _ _ h₁; apply h₁; exact h
+  | ax h => exact Entails.axioms h
+  | mp _ _ ih₁ ih₂ => exact Entails.mp ih₁ ih₂
+
+theorem Consistent.of_satisfiable : Satisfiable Γ → Consistent Γ := by
+  intro ⟨𝓜, ρ, h₁⟩ h₂
+  apply soundness at h₂
+  apply h₂
+  exact h₁
+
+theorem Consistent.empty : Consistent (∅ : 𝓛.FormulaSet n) := by
+  apply of_satisfiable
+  exists ⟨Unit, λ _ _ => (), λ _ _ => True⟩, λ _ => ()
+  intro _ h
+  contradiction
+
+theorem Structure.theory.complete {𝓜 : 𝓛.Structure} : Complete 𝓜.theory := by
+  intro p
+  by_cases h : 𝓜 ⊨ₛ p
+  · exact Or.inl (.hyp h)
+  · exact Or.inr (.hyp h)
+
+theorem Complete.provable_iff_satisfied {𝓣 : 𝓛.Theory} {𝓜 : 𝓣.Model} :
+  Complete 𝓣 → (𝓣 ⊢ p ↔ 𝓜 ⊨ₛ p) := by
+  intro h
+  by_cases h' : 𝓣 ⊢ p <;> simp [h']
+  · apply soundness h'; exact 𝓜.satisfy_theory
+  · cases h p with
+    | inl h => contradiction
+    | inr h => apply soundness h; exact 𝓜.satisfy_theory
+
+namespace Theory
+
+abbrev theorems (𝓣 : 𝓛.Theory) : 𝓛.Theory := { p | 𝓣 ⊢ p }
+
+abbrev Decidable (𝓣 : 𝓛.Theory) := DecidablePred 𝓣.theorems
+
+theorem eq_theory_of_complete {𝓣 : 𝓛.Theory} {𝓜 : 𝓣.Model} :
+  Complete 𝓣 → 𝓣.theorems = 𝓜.theory := by
+  intro h
+  ext p
+  simp [Structure.theory]
+  rw [h.provable_iff_satisfied]
+
+end FirstOrder.Language.Theory
